Impl/JournalistModel.i.dfy
@@ -6,6 +6,7 @@ module JournalistModel {
   import opened DiskLayout
   import opened NativeTypes
   import opened Options
+  import opened Sequences
 
   import opened JournalRanges`Internal
   import opened JournalBytes
@@ -57,7 +58,7 @@ module JournalistModel {
     && 0 <= jm.len1 <= Len()
     && 0 <= jm.len2 <= Len()
     && 0 <= jm.len1 + jm.len2 <= Len()
-    && 0 <= jm.replayIdx as int <= |jm.replayJournal|
+    && 0 <= jm.replayIdx as int <= |jm.replayJournal| <= Len() as int
     && (jm.journalFrontRead.Some? ==>
         JournalRangeOfByteSeq(jm.journalFrontRead.value).Some?)
     && (jm.journalBackRead.Some? ==>
@@ -150,7 +151,23 @@ module JournalistModel {
     && WeightJournalEntries(InMemoryJournal(jm)) == jm.inMemoryWeight as int
   }
 
-  ///// Steps you can take
+  //// Journalist operations
+
+  function {:opaque} JournalistConstructor() : (jm : JournalistModel)
+  ensures Inv(jm)
+  ensures I(jm).inMemoryJournalFrozen == []
+  ensures I(jm).inMemoryJournal == []
+  ensures I(jm).replayJournal == []
+  ensures I(jm).journalFrontRead == None
+  ensures I(jm).journalBackRead == None
+  ensures I(jm).writtenLen == 0
+  {
+    reveal_cyclicSlice();
+    reveal_WeightJournalEntries();
+    JournalistModel(
+        fill(Len() as int, JournalInsert([], [])), // fill with dummies
+        0, 0, 0, [], 0, None, None, 0, 0, 0)
+  }
 
   function {:opaque} hasFrozenJournal(jm: JournalistModel) : (b: bool)
   requires Inv(jm)
@@ -172,6 +189,7 @@ module JournalistModel {
           .(writtenLen := I(jm).writtenLen
                 + |JournalRangeOfByteSeq(s).value|)
   {
+    reveal_WeightJournalEntries();
     var s := marshallJournalEntries(jm.journalEntries, jm.start, jm.len1, jm.frozenJournalBlocks);
     var jm' := jm.(start := basic_mod(jm.start + jm.len1))
                  .(len1 := 0)
@@ -194,6 +212,7 @@ module JournalistModel {
           .(writtenLen := I(jm).writtenLen
                 + |JournalRangeOfByteSeq(s).value|)
   {
+    reveal_WeightJournalEntries();
     var numBlocks := (jm.inMemoryWeight + 4064 - 1) / 4064;
     var s := marshallJournalEntries(jm.journalEntries, jm.start, jm.len2, numBlocks);
     var jm' := jm.(start := 0)
@@ -209,6 +228,20 @@ module JournalistModel {
   ensures len as int == I(jm).writtenLen
   {
     jm.writtenJournalBlocks    
+  }
+
+  function setWrittenJournalLen(jm: JournalistModel, len: uint64)
+      : (jm' : JournalistModel)
+  requires Inv(jm)
+  requires I(jm).inMemoryJournal == []
+  requires I(jm).inMemoryJournalFrozen == []
+  requires 0 <= len <= NumJournalBlocks()
+  ensures Inv(jm')
+  ensures I(jm') == I(jm).(writtenLen := len as int)
+  {
+    reveal_WeightJournalEntries();
+    jm.(writtenJournalBlocks := len)
+      .(frozenJournalBlocks := 0)
   }
 
   /*lemma roundUpOkay(a: int, b: int)
@@ -228,9 +261,70 @@ module JournalistModel {
           .(inMemoryJournalFrozen :=
               I(jm).inMemoryJournalFrozen + I(jm).inMemoryJournal)
   {
+    reveal_WeightJournalEntries();
     jm.(len1 := jm.len1 + jm.len2)
       .(len2 := 0)
       .(frozenJournalBlocks := jm.frozenJournalBlocks + (jm.inMemoryWeight + 4064 - 1) / 4064)
       .(inMemoryWeight := 0)
+  }
+
+  predicate {:opaque} canAppend(jm: JournalistModel, je: JournalEntry)
+  requires Inv(jm)
+  {
+    4064 * (jm.writtenJournalBlocks + jm.frozenJournalBlocks)
+      + jm.inMemoryWeight
+      + WeightJournalEntry(je) as uint64
+      + (if jm.len2 == 0 then 8 else 0)
+        <= 4064 * NumJournalBlocks()
+  }
+
+  lemma lemma_weight_append(a: seq<JournalEntry>, je: JournalEntry)
+  ensures |a| == 0 ==> WeightJournalEntries(a + [je])
+      == WeightJournalEntries(a) + WeightJournalEntry(je) + 8
+  ensures |a| > 0 ==> WeightJournalEntries(a + [je])
+      == WeightJournalEntries(a) + WeightJournalEntry(je)
+  {
+    assert DropLast(a + [je]) == a;
+    assert Last(a + [je]) == je;
+    reveal_WeightJournalEntries();
+    if |a| == 0 {
+      assert WeightJournalEntries(a + [je])
+          == 8 + SumJournalEntries(a) + WeightJournalEntry(je)
+          == 8 + SumJournalEntries([]) + WeightJournalEntry(je)
+          == 8 + WeightJournalEntry(je);
+      assert WeightJournalEntries(a) == 0;
+    }
+  }
+
+  function {:opaque} append(jm: JournalistModel, je: JournalEntry) : (jm' : JournalistModel)
+  requires Inv(jm)
+  requires canAppend(jm, je)
+  ensures
+    && Inv(jm')
+    && I(jm') == I(jm).(inMemoryJournal := I(jm).inMemoryJournal + [je])
+  {
+    lenTimes8LeWeight(InMemoryJournal(jm));
+    lenTimes8LeWeight(InMemoryJournalFrozen(jm));
+
+    var idx := basic_mod(jm.start + jm.len1 + jm.len2);
+    var jm' := jm.(journalEntries := jm.journalEntries[idx as int := je])
+      .(len2 := jm.len2 + 1)
+      .(inMemoryWeight := jm.inMemoryWeight + WeightJournalEntry(je) as uint64 + (if jm.len2 == 0 then 8 else 0));
+
+    assert InMemoryJournal(jm')
+        == InMemoryJournal(jm) + [je] by { reveal_cyclicSlice(); }
+    assert InMemoryJournalFrozen(jm')
+        == InMemoryJournalFrozen(jm) by { reveal_cyclicSlice(); }
+    lemma_weight_append(InMemoryJournal(jm), je);
+    reveal_canAppend();
+
+    jm'
+  }
+
+  function {:opaque} isReplayEmpty(jm: JournalistModel) : (b: bool)
+  requires Inv(jm)
+  ensures b == (I(jm).replayJournal == [])
+  {
+    jm.replayIdx == |jm.replayJournal| as uint64
   }
 }
