Impl/CommitterModel.i.dfy
@@ -1,0 +1,33 @@
+include "../BlockCacheSystem/JournalCache.i.dfy"
+include "JournalistModel.i.dfy"
+include "../lib/DataStructures/MutableMapModel.i.dfy"
+
+// for when you have commitment issues
+
+module CommitterModel {
+  import JournalistModel
+  import MutableMapModel
+  import JC = JournalCache
+  import opened SectorType
+  import opened DiskLayout
+  import opened Options
+  import opened NativeTypes
+
+  datatype CommitterModel = CommitterModel(
+    journalist: JournalistModel.JournalistModel,
+    frozenLoc: Option<Location>,
+    isFrozen: bool,
+
+    frozenJournalPosition: uint64,
+    superblockWrite: Option<JC.ReqId>,
+
+    outstandingJournalWrites: seq<JC.ReqId>,
+
+    superblock: Superblock,
+    newSuperblock: Superblock,
+    whichSuperblock: uint64,
+    commitStatus: JC.CommitStatus,
+
+    syncReqs: MutableMapModel.LinearHashMap<JC.SyncReqStatus>
+  )
+}
